save

DP_Lifting.thy
@@ -1,18 +1,32 @@
 theory DP_Lifting
   imports Main "./Monad"
 begin
-  
+
   (* Types *)
 type_synonym ('a,'M,'b) fun_lifted = "'a \<Rightarrow> ('M,'b) state" ("_ ==_\<Longrightarrow> _" [3,1000,2] 2)
 type_synonym ('a,'b) dpfun = "'a ==('a\<rightharpoonup>'b)\<Longrightarrow> 'b" (infixr "\<Rightarrow>\<^sub>T" 2)
 term 0 (**)
   
   (* Basics *)
-definition fun_app_lifted :: "('M,'a =='M\<Longrightarrow> 'b) state \<Rightarrow> ('M,'a) state \<Rightarrow> ('M,'b) state" (infixl "." 999) where
-  "f\<^sub>T . x\<^sub>T \<equiv> do { f \<leftarrow> f\<^sub>T; x \<leftarrow> x\<^sub>T; f x }"
+notation id ("\<langle>_\<rangle>")
+notation Monad.return ("\<langle>_\<rangle>\<^sub>T")
+
+syntax
+  "_lambda\<^sub>T" :: "[pttrns, 'a] \<Rightarrow> logic" ("(3\<lambda>\<^sub>T_./ _)" [0, 3] 3)
+translations
+  "\<lambda>\<^sub>T v vs. e" \<rightharpoonup> "\<lambda>\<^sub>T v. \<lambda>\<^sub>T vs. e"
+  "\<lambda>\<^sub>T v. e" \<rightharpoonup> "\<lambda> v. \<langle>e\<rangle>\<^sub>T"
+
+definition fun_app :: "('a \<Rightarrow> 'b) \<Rightarrow> 'a \<Rightarrow> 'b" (infixl "." 999) where
+  "fun_app \<equiv> \<lambda> f x. f x"
+term 0 (**)
+  
+definition fun_app_lifted :: "('M,'a =='M\<Longrightarrow> 'b) state \<Rightarrow> ('M,'a) state \<Rightarrow> ('M,'b) state" (infixl ".\<^sub>T" 999) where
+  "f\<^sub>T .\<^sub>T x\<^sub>T \<equiv> do { f \<leftarrow> f\<^sub>T; x \<leftarrow> x\<^sub>T; f x }"
+term 0 (**)
   
 lemma fun_app_lifted_elim:
-  assumes "runState (f\<^sub>T . x\<^sub>T) M = (v, Mv)" "runState f\<^sub>T M = (f, Mf)"
+  assumes "runState (f\<^sub>T .\<^sub>T x\<^sub>T) M = (v, Mv)" "runState f\<^sub>T M = (f, Mf)"
   obtains x Mx where "runState x\<^sub>T Mf = (x, Mx)" and "runState (f x) Mx = (v, Mv)"
   using assms unfolding fun_app_lifted_def bind_def by (auto split: prod.splits)
 term 0 (**)
@@ -21,12 +35,12 @@ definition checkmem :: "'param \<Rightarrow> ('param \<rightharpoonup> 'result, 
   "checkmem param calc \<equiv> do {
     M \<leftarrow> get;
     case M param of
-      Some x \<Rightarrow> \<langle>x\<rangle>
+      Some x \<Rightarrow> return x
     | None \<Rightarrow> do {
         x \<leftarrow> calc;
         M' \<leftarrow> get;
         put (M'(param\<mapsto>x));
-        \<langle>x\<rangle>
+        return x
       }
   }"
   
@@ -34,20 +48,26 @@ abbreviation checkmem_eq :: "('param \<Rightarrow>\<^sub>T 'result) \<Rightarrow
   "(dp\<^sub>T$ param =CHECKMEM= calc) \<equiv> (dp\<^sub>T param = checkmem param calc)"
 term 0 (**)
   
-  (* Auxiliary *)
-syntax
-  "_lambda\<^sub>T" :: "[pttrns, 'a] \<Rightarrow> logic" ("(3\<lambda>\<^sub>T_./ _)" [0, 3] 3)
-translations
-  "\<lambda>\<^sub>T v vs. e" \<rightharpoonup> "\<lambda>\<^sub>T v. \<lambda>\<^sub>T vs. e"
-  "\<lambda>\<^sub>T v. e" \<rightharpoonup> "\<lambda> v. \<langle>e\<rangle>"
-
-definition unlift_' :: "'a \<Rightarrow> ('M, 'a) state" where
-  "unlift_' x \<equiv> \<langle>x\<rangle>"
-definition unlift_3 :: "('a =='M\<Longrightarrow> 'b) \<Rightarrow> ('a \<Rightarrow> ('M, 'b) state)" where
-  "unlift_3 f \<equiv> \<lambda>v0. \<langle>f\<rangle>.\<langle>v0\<rangle>"
-definition unlift_33 :: "('a =='M\<Longrightarrow> 'b =='M\<Longrightarrow> 'c) \<Rightarrow> ('a \<Rightarrow> 'b \<Rightarrow> ('M, 'c) state)" where
-  "unlift_33 f \<equiv> \<lambda>v0 v1. \<langle>f\<rangle>.\<langle>v0\<rangle>.\<langle>v1\<rangle>"
+context
+  includes lifting_syntax
+begin
   
+  (* Auxiliary *)
+definition unlift_' :: "'a \<Rightarrow> ('M, 'a) state" where
+  "unlift_' x \<equiv> \<langle>x\<rangle>\<^sub>T"
+definition unlift_3 :: "('a =='M\<Longrightarrow> 'b) \<Rightarrow> ('a \<Rightarrow> ('M, 'b) state)" where
+  "unlift_3 f \<equiv> \<lambda>v0. \<langle>f\<rangle>\<^sub>T .\<^sub>T \<langle>v0\<rangle>\<^sub>T"
+definition unlift_33 :: "('a =='M\<Longrightarrow> 'b =='M\<Longrightarrow> 'c) \<Rightarrow> ('a \<Rightarrow> 'b \<Rightarrow> ('M, 'c) state)" where
+  "unlift_33 f \<equiv> \<lambda>v0 v1. \<langle>f\<rangle>\<^sub>T .\<^sub>T \<langle>v0\<rangle>\<^sub>T .\<^sub>T \<langle>v1\<rangle>\<^sub>T"
+  
+definition lift_' :: "'a \<Rightarrow> 'a " where
+  "lift_' x \<equiv> x"
+definition lift_3 :: "('a \<Rightarrow> 'b) \<Rightarrow> ('a =='M\<Longrightarrow> 'b)" where
+  "lift_3 f \<equiv> \<lambda>\<^sub>T x. f x"
+definition lift_33 :: "('a \<Rightarrow> 'b \<Rightarrow> 'c) \<Rightarrow> ('a =='M\<Longrightarrow> 'b =='M\<Longrightarrow> 'c)" where
+  "lift_33 f \<equiv> \<lambda>\<^sub>T x0 x1. f x0 x1"
+definition lift_333 :: "('a \<Rightarrow> 'b \<Rightarrow> 'c \<Rightarrow> 'd) \<Rightarrow> ('a =='M\<Longrightarrow> 'b =='M\<Longrightarrow> 'c =='M\<Longrightarrow> 'd)" where
+  "lift_333 f \<equiv> \<lambda>\<^sub>T x0 x1 x2. f x0 x1 x2"
 term 0 (**)
   
   (* HOL *)
@@ -56,7 +76,7 @@ definition If\<^sub>T :: "bool =='M\<Longrightarrow> 'a =='M\<Longrightarrow> 'a
 
 thm comp_def
 definition comp\<^sub>T :: "('b =='M\<Longrightarrow> 'c) =='M\<Longrightarrow> ('a =='M\<Longrightarrow> 'b) =='M\<Longrightarrow> ('a =='M\<Longrightarrow> 'c)" where
-  "comp\<^sub>T \<equiv> \<lambda>\<^sub>T f g. (\<lambda>x. \<langle>f\<rangle> . (\<langle>g\<rangle> . \<langle>x\<rangle>))"
+  "comp\<^sub>T \<equiv> \<lambda>\<^sub>T f g. (\<lambda>x. \<langle>f\<rangle>\<^sub>T .\<^sub>T (\<langle>g\<rangle>\<^sub>T .\<^sub>T \<langle>x\<rangle>\<^sub>T))"
   
 thm id_def
 definition id\<^sub>T :: "'a =='M\<Longrightarrow> 'a" where
@@ -71,19 +91,19 @@ definition case_list\<^sub>T :: "'b =='M\<Longrightarrow> ('a =='M\<Longrightarr
   "case_list\<^sub>T \<equiv> \<lambda>\<^sub>T ifNil ifCons. (\<lambda>val. case_list (unlift_' ifNil) (unlift_33 ifCons) val)"
   
 primrec map\<^sub>T' :: "('a =='M\<Longrightarrow>'b) \<Rightarrow> 'a list =='M\<Longrightarrow> 'b list" where
-  "(map\<^sub>T' f) [] = \<langle>[]\<rangle>"
-| "(map\<^sub>T' f) (x#xs) = \<langle>Cons\<^sub>T\<rangle> . (\<langle>f\<rangle> . \<langle>x\<rangle>) . ((map\<^sub>T' f) xs)"
+  "(map\<^sub>T' f) [] = \<langle>[]\<rangle>\<^sub>T"
+| "(map\<^sub>T' f) (x#xs) = \<langle>Cons\<^sub>T\<rangle>\<^sub>T .\<^sub>T (\<langle>f\<rangle>\<^sub>T .\<^sub>T \<langle>x\<rangle>\<^sub>T) .\<^sub>T ((map\<^sub>T' f) xs)"
 lemma
-  "(map\<^sub>T' f) (x#xs) = \<langle>Cons\<^sub>T\<rangle> . (\<langle>f\<rangle> . \<langle>x\<rangle>) . (\<langle>map\<^sub>T' f\<rangle> . \<langle>xs\<rangle>)" unfolding map\<^sub>T'.simps(2) fun_app_lifted_def left_identity ..
+  "(map\<^sub>T' f) (x#xs) = \<langle>Cons\<^sub>T\<rangle>\<^sub>T .\<^sub>T (\<langle>f\<rangle>\<^sub>T .\<^sub>T \<langle>x\<rangle>\<^sub>T) .\<^sub>T (\<langle>map\<^sub>T' f\<rangle>\<^sub>T .\<^sub>T \<langle>xs\<rangle>\<^sub>T)" unfolding map\<^sub>T'.simps(2) fun_app_lifted_def left_identity ..
     
 definition map\<^sub>T :: "('a =='M\<Longrightarrow> 'b) =='M\<Longrightarrow> 'a list =='M\<Longrightarrow> 'b list" where
   "map\<^sub>T \<equiv> \<lambda>\<^sub>T f\<^sub>T. map\<^sub>T' f\<^sub>T"
   
 primrec fold\<^sub>T' :: "('a =='M\<Longrightarrow> 'b =='M\<Longrightarrow> 'b) \<Rightarrow> 'a list =='M\<Longrightarrow> 'b =='M\<Longrightarrow> 'b" where
-  "(fold\<^sub>T' f) [] = \<langle>id\<^sub>T\<rangle>"
-| "(fold\<^sub>T' f) (x#xs) = \<langle>comp\<^sub>T\<rangle> . ((fold\<^sub>T' f) xs) . (\<langle>f\<rangle> . \<langle>x\<rangle>)"
+  "(fold\<^sub>T' f) [] = \<langle>id\<^sub>T\<rangle>\<^sub>T"
+| "(fold\<^sub>T' f) (x#xs) = \<langle>comp\<^sub>T\<rangle>\<^sub>T .\<^sub>T ((fold\<^sub>T' f) xs) .\<^sub>T (\<langle>f\<rangle>\<^sub>T .\<^sub>T \<langle>x\<rangle>\<^sub>T)"
 lemma
-  "(fold\<^sub>T' f) (x#xs) = \<langle>comp\<^sub>T\<rangle> . (\<langle>fold\<^sub>T' f\<rangle> . \<langle>xs\<rangle>) . (\<langle>f\<rangle> . \<langle>x\<rangle>)" unfolding fold\<^sub>T'.simps(2) fun_app_lifted_def left_identity ..
+  "(fold\<^sub>T' f) (x#xs) = \<langle>comp\<^sub>T\<rangle>\<^sub>T .\<^sub>T (\<langle>fold\<^sub>T' f\<rangle>\<^sub>T .\<^sub>T \<langle>xs\<rangle>\<^sub>T) .\<^sub>T (\<langle>f\<rangle>\<^sub>T .\<^sub>T \<langle>x\<rangle>\<^sub>T)" unfolding fold\<^sub>T'.simps(2) fun_app_lifted_def left_identity ..
     
 definition fold\<^sub>T :: "('a =='M\<Longrightarrow> 'b =='M\<Longrightarrow> 'b) =='M\<Longrightarrow> 'a list =='M\<Longrightarrow> 'b =='M\<Longrightarrow> 'b" where
   "fold\<^sub>T \<equiv> \<lambda>\<^sub>T f\<^sub>T. fold\<^sub>T' f\<^sub>T"
@@ -107,7 +127,7 @@ definition Pair\<^sub>T :: "'a0 =='M\<Longrightarrow> 'a1 =='M\<Longrightarrow> 
 definition case_prod\<^sub>T :: "('a0 =='M\<Longrightarrow> 'a1 =='M\<Longrightarrow> 'b) =='M\<Longrightarrow> ('a0\<times>'a1) =='M\<Longrightarrow> 'b" where
   "case_prod\<^sub>T \<equiv> \<lambda>\<^sub>T ifProd. (\<lambda>val. case_prod (unlift_33 ifProd) val)"
   
-term "\<langle>case_prod\<^sub>T\<rangle> . \<langle>\<lambda>\<^sub>T v0 v1. v0+v1\<rangle> . (\<langle>Pair\<^sub>T\<rangle> . \<langle>0\<rangle> . \<langle>0::int\<rangle>)"
+term "\<langle>case_prod\<^sub>T\<rangle>\<^sub>T .\<^sub>T \<langle>\<lambda>\<^sub>T v0 v1. v0+v1\<rangle>\<^sub>T .\<^sub>T (\<langle>Pair\<^sub>T\<rangle>\<^sub>T .\<^sub>T \<langle>0\<rangle>\<^sub>T .\<^sub>T \<langle>0::int\<rangle>\<^sub>T)"
 term 0 (**)
   
   (* Arithmetic *)
@@ -120,4 +140,5 @@ definition max\<^sub>T :: "'a::ord =='M\<Longrightarrow> 'a =='M\<Longrightarrow
 definition plus\<^sub>T :: "'a::plus =='M\<Longrightarrow> 'a =='M\<Longrightarrow> 'a" where
   "plus\<^sub>T \<equiv> \<lambda>\<^sub>T x y. plus x y"
 term 0 (**)
+end
 end
